src/Std/Data/HashSet/Raw.lean
@@ -229,16 +229,10 @@ section Unverified
 /-! We currently do not provide lemmas for the functions below. -/
 
 /-- Check if all elements satisfy the predicate, short-circuiting if a predicate fails. -/
-@[inline] def all (m : Raw α) (p : α → Bool) : Bool := Id.run do
-  for a in m do
-    if ¬ p a then return false
-  return true
+@[inline] def all (m : Raw α) (p : α → Bool) : Bool := m.inner.all (fun a _ => p a)
 
 /-- Check if any element satisfies the predicate, short-circuiting if a predicate succeeds. -/
-@[inline] def any (m : Raw α) (p : α → Bool) : Bool := Id.run do
-  for a in m do
-    if p a then return true
-  return false
+@[inline] def any (m : Raw α) (p : α → Bool) : Bool := m.inner.any (fun a _ => p a)
 
 /--
 Inserts multiple mappings into the hash set by iterating over the given collection and calling
